

The Fourier Series & Transforms

Equation	Discrete Time	Continuous Time
Fourier Series (Analysis)	$X_k = \frac{1}{N} \sum_{n \in \langle N \rangle} x(n) e^{-ik\omega_0 n}$	$X_k = \frac{1}{T} \int_{\langle T \rangle} x(t) e^{-ik\omega_0 t} dt$
Inverse Fourier Series (Synthesis)	$x(n) = \sum_{k \in \langle N \rangle} X_k e^{ik\omega_0 n}$	$x(t) = \sum_{k=-\infty}^{\infty} X_k e^{ik\omega_0 t}$
DFT (Analysis)	$X[k] = \frac{1}{N} \sum_{n=0}^{N-1} x(n) e^{-ik\omega_0 n}$	N/A
Inverse DFT (Synthesis)	$x(n) = \sum_{k=0}^{N-1} X[k] e^{ik\omega_0 n}$	N/A
Fourier Transform (Analysis)	$X(\omega) = \sum_{n=-\infty}^{\infty} x(n) e^{-i\omega n}$	$X(\omega) = \int_{-\infty}^{\infty} x(t) e^{-i\omega t} dt$
Inverse Fourier Transform (Synthesis)	$x(n) = \frac{1}{2\pi} \int_{\langle 2\pi \rangle} X(\omega) e^{i\omega n} d\omega$	$x(t) = \frac{1}{2\pi} \int_{-\infty}^{\infty} X(\omega) e^{i\omega t} d\omega$
Z-Transform	$X(z) = \sum_{n=-\infty}^{\infty} x(n) z^{-n}$	N/A

Note: $\langle p \rangle$ represents a period of p (e.g. $(-\frac{1}{2}p, \frac{1}{2}p)$ or $(0, p)$). For the equations, $\omega \leftrightarrow 2\pi f$, $\omega_0 \leftrightarrow 2\pi f_0$, and $T = \frac{1}{f_0} = \frac{2\pi}{\omega_0}$ or $N = \frac{1}{f_0} = \frac{2\pi}{\omega_0}$.

Fourier Series Properties

Property	DTFS	CTFS
Linearity	$\alpha x(n) \xleftrightarrow{\mathcal{F}} \alpha X_k$ $x(n) + y(n) \xleftrightarrow{\mathcal{F}} X_k + Y_k$	$\alpha x(t) \xleftrightarrow{\mathcal{F}} \alpha X_k$ $x(t) + y(t) \xleftrightarrow{\mathcal{F}} X_k + Y_k$
Convolution	$(x * y)(n) \xleftrightarrow{\mathcal{F}} X_k \cdot Y_k$	$(x * y)(t) \xleftrightarrow{\mathcal{F}} X_k \cdot Y_k$
Time Reversal	$x(-n) \xleftrightarrow{\mathcal{F}} X_{-k}$	$x(-t) \xleftrightarrow{\mathcal{F}} X_{-k}$
Conjugation	$x^*(n) \xleftrightarrow{\mathcal{F}} X_{-k}^*$	$x^*(t) \xleftrightarrow{\mathcal{F}} X_{-k}^*$
Conjugate Symmetry	$x(n) \in \mathbb{R} \iff X_k = X_{-k}^*$	$x(t) \in \mathbb{R} \iff X_k = X_{-k}^*$
Real and Even x	Real and even X_k	
Real and Odd x	Imaginary and odd X_k	
Imaginary and Even x	Imaginary and even X_k	
Imaginary and Odd x	Real and odd X_k	
Time Shift	$x(n - n_0) \xleftrightarrow{\mathcal{F}} e^{-ik\omega_0 n_0} X_k$	$x(t - t_0) \xleftrightarrow{\mathcal{F}} e^{-ik\omega_0 t_0} X_k$
Parseval's	$\frac{1}{N} \sum_{n \in \langle N \rangle} x(n) ^2 = \sum_{k \in \langle N \rangle} X_k ^2$	$\frac{1}{T} \int_{\langle T \rangle} x(t) ^2 dt = \sum_{k=-\infty}^{\infty} X_k ^2$
Poisson's	$\sum_{l=-\infty}^{\infty} \delta(n - lN) = \frac{1}{N} \sum_{k \in \langle N \rangle} e^{ik\omega_0 n}$	$\sum_{l=-\infty}^{\infty} \delta(t - lT) = \frac{1}{T} \sum_{k=-\infty}^{\infty} e^{ik\omega_0 t}$

Fourier Transform Pairs

Pairs	Discrete Time	Continuous Time
Constant	$1 \xleftrightarrow{\mathcal{F}} 2\pi \sum_{k=-\infty}^{\infty} \delta(\omega - 2\pi k)$	$1 \xleftrightarrow{\mathcal{F}} 2\pi \delta(\omega)$
Complex Exponential	$e^{i\omega_0 n} \xleftrightarrow{\mathcal{F}} 2\pi \sum_{k=-\infty}^{\infty} \delta(\omega - \omega_0 - 2\pi k)$	$e^{i\omega_0 t} \xleftrightarrow{\mathcal{F}} 2\pi \delta(\omega - \omega_0)$
Exponential	$\alpha^n u(n) \xleftrightarrow{\mathcal{F}} \frac{1}{1 - \alpha e^{-i\omega}}, \alpha < 1$	$e^{-\alpha t} u(t) \xleftrightarrow{\mathcal{F}} \frac{1}{i\omega + \alpha}, \Re(\alpha) > 0$
Delta	$\delta(n) \xleftrightarrow{\mathcal{F}} 1$	$\delta(t) \xleftrightarrow{\mathcal{F}} 1$
Shifted Delta	$\delta(n - n_0) \xleftrightarrow{\mathcal{F}} e^{-i\omega n_0}$	$\delta(t - t_0) \xleftrightarrow{\mathcal{F}} e^{-i\omega t_0}$
Rect in Time	$x(n) = \begin{cases} 1 & n \in \{-M, \dots, M\} \\ 0 & \text{otherwise} \end{cases}$ $X(\omega) = \begin{cases} \frac{\sin((\frac{2M+1}{2})\omega)}{\sin(\omega/2)} & \omega \neq 0 \\ 2M+1 & \omega = 0 \end{cases}$	$x(t) = \begin{cases} 1 & t \leq B \\ 0 & t > B \end{cases}$ $X(\omega) = 2B \operatorname{sinc}\left(\frac{B}{\pi}\omega\right)$
Rect in Freq.	$f(n) = \frac{\omega_0}{\pi} \operatorname{sinc}\left(\frac{\omega_0}{\pi}n\right)$ $F(\omega) = \begin{cases} 1 & \omega \in [-\omega_0 + 2\pi k, \omega_0 + 2\pi k] \\ 0 & \text{otherwise} \end{cases}$	$f(t) = \frac{\omega_0}{\pi} \operatorname{sinc}\left(\frac{\omega_0}{\pi}t\right)$ $F(\omega) = \begin{cases} 1 & \omega \in [-\omega_0, \omega_0] \\ 0 & \text{otherwise} \end{cases}$
Delta Train	$s(n) = \sum_{l=-\infty}^{\infty} \delta(n - lN)$ $S(\omega) = \frac{2\pi}{N} \sum_{k=-\infty}^{\infty} \delta(\omega - k\frac{2\pi}{N})$	$s(t) = \sum_{l=-\infty}^{\infty} \delta(t - lT)$ $S(\omega) = \frac{2\pi}{T} \sum_{k=-\infty}^{\infty} \delta(\omega - k\frac{2\pi}{T})$

Note: $\omega = 2\pi f$.

Important Equations

Name	Equation
Sinc	$\operatorname{sinc}(x) = \begin{cases} \frac{\sin(\pi x)}{\pi x} & x \neq 0 \\ 1 & x = 0 \end{cases}$
Euler's	$e^{i\omega} = \cos(\omega) + i \sin(\omega)$
Inverse Euler's	$\cos(\omega) = \frac{1}{2} (e^{i\omega} + e^{-i\omega})$ $\sin(\omega) = \frac{1}{2i} (e^{i\omega} - e^{-i\omega})$
Infinite Geometric Series Summation	$\sum_{k=0}^{\infty} ar^k = \frac{a}{1-r} \quad r < 1$
Finite Geometric Series Summation	$\sum_{k=0}^n ar^k = \frac{a - ar^{n+1}}{1-r} \quad r \neq 1$

Fourier Transform Properties

Property	DTFT	CTFT
Linearity	$\alpha x(n) \xleftrightarrow{\mathcal{F}} \alpha X(\omega)$ $x(n) + y(n) \xleftrightarrow{\mathcal{F}} X(\omega) + Y(\omega)$	$\alpha x(t) \xleftrightarrow{\mathcal{F}} \alpha X(\omega)$ $x(t) + y(t) \xleftrightarrow{\mathcal{F}} X(\omega) + Y(\omega)$
Convolution	$(x * y)(n) \xleftrightarrow{\mathcal{F}} X(\omega)Y(\omega)$	$(x * y)(t) \xleftrightarrow{\mathcal{F}} X(\omega)Y(\omega)$
Modulation	$x(n)y(n) \xleftrightarrow{\mathcal{F}} \frac{1}{2\pi}(X \circledast Y)(\omega)$	$x(t)y(t) \xleftrightarrow{\mathcal{F}} \frac{1}{2\pi}(X * Y)(\omega)$
Downsampling	$x(an) \xleftrightarrow{\mathcal{F}} \frac{1}{a} \sum_{k=0}^{a-1} X\left(\frac{\omega - 2k\pi}{a}\right), a \in \mathbb{Z}^+$	$x(at) \xleftrightarrow{\mathcal{F}} \frac{1}{ a } X\left(\frac{\omega}{a}\right)$
Upsampling	$\begin{cases} x\left(\frac{n}{a}\right) & a \mid n \\ 0 & a \nmid n \end{cases} \xleftrightarrow{\mathcal{F}} X(a\omega), a \in \mathbb{Z}^+$	$x\left(\frac{t}{a}\right) \xleftrightarrow{\mathcal{F}} a X(a\omega)$
Time-Reversal	$x(-n) \xleftrightarrow{\mathcal{F}} X(-\omega)$	$x(-t) \xleftrightarrow{\mathcal{F}} X(-\omega)$
Conjugation	$x^*(n) \xleftrightarrow{\mathcal{F}} X^*(-\omega)$	$x^*(t) \xleftrightarrow{\mathcal{F}} X^*(-\omega)$
Conjugate Symmetry	$x(n) \in \mathbb{R} \iff X(\omega) = X^*(-\omega)$	$x(t) \in \mathbb{R} \iff X(\omega) = X^*(-\omega)$
Real and Even x	Real and even $X(\omega)$	
Real and Odd x	Imaginary and odd $X(\omega)$	
Imaginary and Even x	Imaginary and even $X(\omega)$	
Imaginary and Odd x	Real and odd $X(\omega)$	
Time Shift	$x(n - n_0) \xleftrightarrow{\mathcal{F}} e^{-i\omega n_0} X(\omega)$	$x(t - t_0) \xleftrightarrow{\mathcal{F}} e^{-i\omega t_0} X(\omega)$
Frequency Shift	$e^{i\omega_0 n} x(n) \xleftrightarrow{\mathcal{F}} X(\omega - \omega_0)$	$e^{i\omega_0 t} x(t) \xleftrightarrow{\mathcal{F}} X(\omega - \omega_0)$
Time Differentiation	N/A	$\frac{d}{dt}x(t) \xleftrightarrow{\mathcal{F}} i\omega X(\omega)$
Freq. Differentiation	$nx(n) \xleftrightarrow{\mathcal{F}} i\frac{d}{d\omega}X(\omega)$	$tx(t) \xleftrightarrow{\mathcal{F}} i\frac{d}{d\omega}X(\omega)$
Accumulation/Integration	$\sum_{k=-\infty}^n x(k) \xleftrightarrow{\mathcal{F}} \pi X(0) \frac{X(\omega)}{1 - e^{-i\omega}} + \sum_{k=-\infty}^{\infty} \delta(\omega - 2\pi k)$	$\int_{-\infty}^t x(\tau) d\tau \xleftrightarrow{\mathcal{F}} \frac{X(\omega)}{i\omega} + \pi X(0)\delta(\omega)$
Parseval's	$\sum_{n=-\infty}^{\infty} x(n) ^2 = \frac{1}{2\pi} \int_{\langle 2\pi \rangle} X(\omega) ^2 d\omega$	$\int_{-\infty}^{\infty} x(t) ^2 dt = \frac{1}{2\pi} \int_{-\infty}^{\infty} X(\omega) ^2 d\omega$
Duality	$\textcolor{blue}{x(n)} \xleftrightarrow{\text{DTFT}} \textcolor{red}{X(\omega)}$ $\textcolor{red}{X(t)} \xleftrightarrow{\text{CTFS } p=2\pi} \textcolor{blue}{X_k} = \textcolor{blue}{x(-k)}$	$\textcolor{blue}{x(t)} \xleftrightarrow{\mathcal{F}} \textcolor{red}{X(\omega)}$ $\textcolor{red}{X(t)} \xleftrightarrow{\mathcal{F}} 2\pi \textcolor{blue}{x(-\omega)}$

Note: $(X \circledast Y)(\omega)$ is the circular, or periodic convolution of $X(\omega)$ and $Y(\omega)$. This is equivalent to convolving $Y(\omega)$ with one 2π period of $X(\omega)$ (and the rest of $X(\omega)$ zeroed out), or vice versa. $a \mid n$ means n is divisible by a , and $a \nmid n$ means n is not divisible by a .

Z-Transform Properties & Pairs

Property	Z-Transform	Region of Convergence
Linearity	$\alpha x(n) + \beta y(n) \xleftrightarrow{\mathcal{Z}} \alpha X(z) + \beta Y(z)$	$\supseteq \text{RoC}(x) \cap \text{RoC}(y)$
Time Shift	$x(n - n_0) \xleftrightarrow{\mathcal{Z}} z^{-n_0} X(z)$	$\text{RoC}(x)$ except $\begin{cases} z = 0 & n_0 > 0 \\ z = \infty & n_0 < 0 \end{cases}$
z Scaling	$a^n x(n) \xleftrightarrow{\mathcal{Z}} X\left(\frac{z}{a}\right)$	$ a \cdot \text{RoC}(x)$
Time Reversal	$x(-n) \xleftrightarrow{\mathcal{Z}} X(z^{-1})$	$1/\text{RoC}(x)$
Convolution	$(x * h)(n) \xleftrightarrow{\mathcal{Z}} X(z)H(z)$	$\supseteq \text{RoC}(x) \cap \text{RoC}(h)$
Conjugation	$x^*(n) \xleftrightarrow{\mathcal{Z}} X^*(z^*)$	$\text{RoC}(x)$
Conjugate Symmetry	$x(n) \in \mathbb{R} \xleftrightarrow{\mathcal{F}} X(z) = X^*(z^*)$	$\text{RoC}(x)$
z Differentiation	$nx(n) \xleftrightarrow{\mathcal{Z}} -z \frac{dX(z)}{dz}$	$\text{RoC}(x)$
Initial Value Theorem	$x(n) = 0, \forall n < 0 \xleftrightarrow{\mathcal{Z}} \lim_{z \rightarrow \infty} X(z) = x(0)$	Outside the outermost pole, out to, and including, $+\infty$

Signal	Z-Transform	Region of Convergence
$\delta(n)$	1	$\{z \in \mathbb{C}\}$
$\delta(n - n_0)$	z^{-n_0}	$\{z \in \mathbb{C}\}$ except $\begin{cases} z = 0 & n_0 > 0 \\ z = \infty & n_0 < 0 \end{cases}$
$u(n)$	$\frac{1}{1-z^{-1}}$	$\{z \in \mathbb{C} \mid z > 1\}$
$-u(-n - 1)$	$\frac{1}{1-z^{-1}}$	$\{z \in \mathbb{C} \mid z < 1\}$
$a^n u(n)$	$\frac{1}{1-az^{-1}}$	$\{z \in \mathbb{C} \mid z > a \}$
$-a^n u(-n - 1)$	$\frac{1}{1-az^{-1}}$	$\{z \in \mathbb{C} \mid z < a \}$
$na^n u(n)$	$\frac{az^{-1}}{(1-az^{-1})^2}$	$\{z \in \mathbb{C} \mid z > a \}$
$-na^n u(-n - 1)$	$\frac{az^{-1}}{(1-az^{-1})^2}$	$\{z \in \mathbb{C} \mid z < a \}$
$\cos(\omega_0 n)u(n)$	$\frac{1 - \cos(\omega_0)z^{-1}}{1 - 2\cos(\omega_0)z^{-1} + z^{-2}}$	$\{z \in \mathbb{C} \mid z > 1\}$
$\sin(\omega_0 n)u(n)$	$\frac{\sin(\omega_0)z^{-1}}{1 - 2\cos(\omega_0)z^{-1} + z^{-2}}$	$\{z \in \mathbb{C} \mid z > 1\}$
$a^n \cos(\omega_0 n)u(n)$	$\frac{1 - a\cos(\omega_0)z^{-1}}{1 - 2a\cos(\omega_0)z^{-1} + a^2z^{-2}}$	$\{z \in \mathbb{C} \mid z > a \}$
$a^n \sin(\omega_0 n)u(n)$	$\frac{a\sin(\omega_0)z^{-1}}{1 - 2a\cos(\omega_0)z^{-1} + a^2z^{-2}}$	$\{z \in \mathbb{C} \mid z > a \}$